examples/machine-code/instruction-set-models/x86_64/x64_Script.sml
@@ -22,8 +22,8 @@ val x64_decode_bytes_def = Define `
 val x64_execute_some_def = Define `
   x64_execute_some i w s = option_apply (x64_execute iiid_dummy i w s) (\t. SOME (SND t))`;
 
-val Z64_NEXT_def = Define `
-  Z64_NEXT s =
+val X64_NEXT_def = Define `
+  X64_NEXT s =
     let e = ZREAD_RIP s in                                     (* read rip *)
     let xs = MAP THE (ZREAD_INSTR_BYTES 20 e s) in             (* read next 20 bytes *)
     let m = x64_decode_bytes xs in                             (* attempt to decode *)
@@ -33,19 +33,19 @@ val Z64_NEXT_def = Define `
           if EVERY (\x. ~(x = NONE)) (ZREAD_INSTR_BYTES n e s) (* check that the memory is there *)
           then x64_execute_some i (n2w n) s else NONE          (* execute the instruction *)`;
 
-val Z64_NEXT_REL_def = Define `
-  Z64_NEXT_REL s t = ?u. Z64_ICACHE s u /\ (Z64_NEXT u = SOME t)`;
+val X64_NEXT_REL_def = Define `
+  X64_NEXT_REL s t = ?u. X64_ICACHE s u /\ (X64_NEXT u = SOME t)`;
 
 
-(* help to evaluate Z64_NEXT *)
+(* help to evaluate X64_NEXT *)
 
-val Z64_NEXT_THM = store_thm("Z64_NEXT_THM",
+val X64_NEXT_THM = store_thm("X64_NEXT_THM",
   ``(x64_decode xs = SOME (i,w)) ==>
     (FOLDR APPEND [] (MAP w2bits (MAP THE (ZREAD_INSTR_BYTES 20 (ZREAD_RIP s) s))) = xs) ==>
     (EVERY (\x. ~(x = NONE)) (ZREAD_INSTR_BYTES (20 - (LENGTH w DIV 8)) (ZREAD_RIP s) s)) ==>
     (x64_execute iiid_dummy i (n2w (20 - (LENGTH w DIV 8))) s = SOME (tt,s')) ==>
-    (Z64_NEXT s = SOME s')``,
-  SIMP_TAC std_ss [Z64_NEXT_def,LET_DEF,ZREAD_REG_def,x64_decode_bytes_def,
+    (X64_NEXT s = SOME s')``,
+  SIMP_TAC std_ss [X64_NEXT_def,LET_DEF,ZREAD_REG_def,x64_decode_bytes_def,
     x64_execute_some_def,option_apply_def]);
 
 
